refactor: lake: generalize targets (squashed WIP)
* refactor: unify facet data
* feat: generalize build keys
* refactor: generalize families
* refactor: generalize facet config
* chore: facet configs for all facets
* chore: touchups
* feat: full `BuildKey.fetch`  & support
* refactor: generalize build info
* refactor: remove facet kind from key
* refactor:  generalize workspace facet configs
* chore: minor touchups
* chore: minor touchups
* chore: facet kind constants & touch-ups

src/lake/Lake/Build/Data.lean
@@ -15,59 +15,102 @@ namespace Lake
 --------------------------------------------------------------------------------
 
 /--
-The open type family which maps a module facet's name to its build data
-in the Lake build store. For example, a transitive × direct import pair
-for the `lean.imports` facet or an active build target for `lean.c`.
-
-It is an open type, meaning additional mappings can be add lazily
-as needed (via `module_data`).
--/
-opaque ModuleData (facet : Name) : Type
-
-/--
-The open type family which maps a package facet's name to its build data
-in the Lake build store. For example, a transitive dependencies of the package
-for the facet `deps`.
-
-It is an open type, meaning additional mappings can be add lazily
-as needed (via `package_data`).
--/
-opaque PackageData (facet : Name) : Type
-
-/--
-The open type family which maps a (builtin) Lake target's (e.g., `extern_lib`)
-facet to its associated build data. For example, an active build target for
-the `externLib.static` facet.
+The open type family which maps a Lake target to its associated build data.
+For example, the generated static library for the `externLib.static` facet of
+an external library.
 
 It is an open type, meaning additional mappings can be add lazily
 as needed (via `target_data`).
 -/
-opaque TargetData (facet : Name) : Type
+opaque TargetData (name : Name) : Type
 
-/-
-The open type family which maps a library facet's name to its build data
-in the Lake build store. For example, an active build target for the `static`
-facet.
+/--
+The open type family which maps a facet to its build data in
+the Lake build store. For example, the imports of a module.
+
+It is an open type, meaning additional mappings can be add lazily
+as needed (via `facet_data`).
+-/
+abbrev FacetData (kind facet : Name) := TargetData (kind ++ facet)
+
+instance [h : FamilyDef TargetData (kind ++ facet) α] : FamilyDef (FacetData kind) facet α :=
+  ⟨h.fam_eq⟩
+
+/--
+The open type family which maps a module facet's name to its build data
+in the Lake build store. For example, the generated C file for `c`.
+
+It is an open type, meaning additional mappings can be add lazily
+as needed (via `module_data`).
+-/
+abbrev ModuleData := FacetData Module.facetKind
+
+/--
+The open type family which maps a package facet's name to its build data
+in the Lake build store. For example, the direct dependencies of the package
+for the `deps` facet.
+
+It is an open type, meaning additional mappings can be add lazily
+as needed (via `package_data`).
+-/
+abbrev PackageData := FacetData Package.facetKind
+
+/-- The kind identifier for facets of a Lean library. -/
+abbrev LeanLib.facetKind : Name := `leanLib
+
+/--
+The open type family which maps a Lean library facet's name to its build data
+in the Lake build store. For example, the generated static library for the
+`static` facet.
 
 It is an open type, meaning additional mappings can be add lazily
 as needed (via `library_data`).
 -/
-abbrev LibraryData (facet : Name) := TargetData (`leanLib ++ facet)
+abbrev LibraryData := FacetData LeanLib.facetKind
 
-instance [h : FamilyOut LibraryData facet α] : FamilyDef TargetData (`leanLib ++ facet) α :=
-  ⟨by simp [h.family_key_eq_type]⟩
+@[inherit_doc LibraryData]
+abbrev LeanLibData := LibraryData
 
-instance [h : FamilyOut TargetData (`leanLib ++ facet) α] : FamilyDef LibraryData facet α :=
-  ⟨h.family_key_eq_type⟩
+/-- The kind identifier for facets of a Lean executable. -/
+abbrev LeanExe.facetKind : Name := `leanExe
 
 /--
-The open type family which maps a custom target (package × target name) to
-its build data in the Lake build store.
+The type family which maps a Lean executable facet's name to its build data
+in the Lake build store. For example, the generated executable for the
+`exe` facet.
+-/
+abbrev LeanExeData := FacetData LeanExe.facetKind
+
+/-- The kind identifier for facets of an external library. -/
+abbrev ExternLib.facetKind : Name := `externLib
+
+/--
+The type family which maps an external library facet's name to its build data
+in the Lake build store. For example, the generated static library for the
+`static` facet.
+-/
+abbrev ExternLibData := FacetData ExternLib.facetKind
+
+/--
+The open type family which maps a custom package target
+(package × target name) to its build data in the Lake build store.
 
 It is an open type, meaning additional mappings can be add lazily
 as needed (via `custom_data`).
 -/
-opaque CustomData (target : Name × Name) : Type
+opaque CustomDataFam (target : Name × Name) : Type
+
+/--
+The open type family which maps a custom package target
+to its build data in the Lake build store.
+
+It is an open type, meaning additional mappings can be add lazily
+as needed (via `custom_data`).
+-/
+abbrev CustomData (package target : Name) := CustomDataFam (package, target)
+
+instance [h : FamilyDef CustomDataFam (p, t) α] : FamilyDef (CustomData p) t α :=
+  ⟨h.fam_eq⟩
 
 --------------------------------------------------------------------------------
 /-! ## Build Data                                                             -/
@@ -79,55 +122,90 @@ It is a simple type function composed of the separate open type families for
 modules facets, package facets, Lake target facets, and custom targets.
 -/
 abbrev BuildData : BuildKey → Type
-| .moduleFacet _ f => ModuleData f
-| .packageFacet _ f => PackageData f
-| .targetFacet _ _ f => TargetData f
-| .customTarget p t => CustomData (p, t)
+| .module _ => TargetData Module.facetKind
+| .package _ => TargetData Package.facetKind
+| .packageTarget p t .anonymous => CustomData p t
+| .packageTarget _ _ k => TargetData k
+| .facet t f => FacetData t.kind f
 
-instance (priority := low) : FamilyDef BuildData k (BuildData k) := ⟨rfl⟩
 instance (priority := low) : FamilyDef BuildData (.moduleFacet m f) (ModuleData f) := ⟨rfl⟩
 instance (priority := low) : FamilyDef BuildData (.packageFacet p f) (PackageData f) := ⟨rfl⟩
-instance (priority := low) : FamilyDef BuildData (.targetFacet p t f) (TargetData f) := ⟨rfl⟩
-instance (priority := low) : FamilyDef BuildData (.customTarget p t) (CustomData (p,t)) := ⟨rfl⟩
+instance (priority := low) : FamilyDef BuildData (.customTarget p t) (CustomData p t) := ⟨rfl⟩
+instance (priority := low) : FamilyDef BuildData (.facet t f) (FacetData t.kind f) := ⟨rfl⟩
+instance (priority := low) : FamilyDef BuildData (.targetFacet p t LeanLib.facetKind f) (LeanLibData f) := ⟨rfl⟩
+instance (priority := low) : FamilyDef BuildData (.targetFacet p t LeanExe.facetKind f) (LeanExeData f) := ⟨rfl⟩
+instance (priority := low) : FamilyDef BuildData (.targetFacet p t ExternLib.facetKind f) (ExternLibData f) := ⟨rfl⟩
+
+instance [FamilyOut TargetData Module.facetKind α]
+: FamilyDef BuildData (.module k) α where
+  fam_eq := by unfold BuildData; simp
+
+instance [FamilyOut TargetData Package.facetKind α]
+: FamilyDef BuildData (.package k) α where
+  fam_eq := by unfold BuildData; simp
+
+instance [FamilyOut TargetData LeanLib.facetKind α]
+: FamilyDef BuildData (.packageTarget p t LeanLib.facetKind) α where
+  fam_eq := by unfold BuildData; simp
+
+instance [FamilyOut TargetData LeanExe.facetKind α]
+: FamilyDef BuildData (.packageTarget p t LeanExe.facetKind) α where
+  fam_eq := by unfold BuildData; simp
+
+instance [FamilyOut TargetData ExternLib.facetKind α]
+: FamilyDef BuildData (.packageTarget p t ExternLib.facetKind) α where
+  fam_eq := by unfold BuildData; simp
+
+theorem BuildKey.data_eq_of_kind {k : BuildKey} :
+  ¬ k.kind.isAnonymous → (BuildData k) = TargetData k.kind
+:= by unfold BuildData; split <;> simp [BuildKey.kind, Lean.Name.isAnonymous]
 
 --------------------------------------------------------------------------------
 /-! ## Macros for Declaring Build Data                                        -/
 --------------------------------------------------------------------------------
 
+open Parser Command
+
+/-- Macro for declaring new `FacetData`. -/
+scoped macro (name := facetDataDecl)
+  doc?:optional(docComment) "facet_data " kind:ident facet:ident " : " ty:term
+: command => do
+  let fam := mkCIdentFrom (← getRef) ``TargetData
+  let kindName := Name.quoteFrom kind kind.getId
+  let facetName := Name.quoteFrom facet facet.getId
+  let id := mkIdentFrom facet (canonical := true) <|
+    facet.getId.modifyBase (kind.getId ++ ·)
+  `($[$doc?]? family_def $id : $fam ($kindName ++ $facetName) := $ty)
+
 /-- Macro for declaring new `PackageData`. -/
-scoped macro (name := packageDataDecl) doc?:optional(Parser.Command.docComment)
-"package_data " id:ident " : " ty:term : command => do
-  let dty := mkCIdentFrom (← getRef) ``PackageData
-  let key := Name.quoteFrom id id.getId
-  `($[$doc?]? family_def $id : $dty $key := $ty)
+scoped macro (name := packageDataDecl)
+  doc?:optional(docComment) "package_data " facet:ident " : " ty:term
+: command => `($[$doc?]? facet_data $(mkIdent Package.facetKind) $facet : $ty)
 
 /-- Macro for declaring new `ModuleData`. -/
-scoped macro (name := moduleDataDecl) doc?:optional(Parser.Command.docComment)
-"module_data " id:ident " : " ty:term : command => do
-  let dty := mkCIdentFrom (← getRef) ``ModuleData
-  let key := Name.quoteFrom id id.getId
-  `($[$doc?]? family_def $id : $dty $key := $ty)
+scoped macro (name := moduleDataDecl)
+  doc?:optional(docComment) "module_data " facet:ident " : " ty:term
+: command => `($[$doc?]? facet_data $(mkIdent Module.facetKind) $facet : $ty)
 
-/-- Macro for declaring new `TargetData` for libraries. -/
-scoped macro (name := libraryDataDecl) doc?:optional(Parser.Command.docComment)
-"library_data " id:ident " : " ty:term : command => do
-  let dty := mkCIdentFrom (← getRef) ``TargetData
-  let key := Name.quoteFrom id id.getId
-  let id := mkIdentFrom id (canonical := true) <| id.getId.modifyBase (`leanLib ++ ·)
-  `($[$doc?]? family_def $id : $dty (`leanLib ++ $key) := $ty)
+/-- Macro for declaring new `LibraryData`. -/
+scoped macro (name := libraryDataDecl)
+  doc?:optional(docComment) "library_data " facet:ident " : " ty:term
+: command => `($[$doc?]? facet_data $(mkIdent LeanLib.facetKind) $facet : $ty)
 
 /-- Macro for declaring new `TargetData`. -/
-scoped macro (name := targetDataDecl) doc?:optional(Parser.Command.docComment)
-"target_data " id:ident " : " ty:term : command => do
-  let dty := mkCIdentFrom (← getRef) ``TargetData
-  let key := Name.quoteFrom id id.getId
-  `($[$doc?]? family_def $id : $dty $key := $ty)
+scoped macro (name := targetDataDecl)
+  doc?:optional(docComment) "target_data " id:ident " : " ty:term
+: command => do
+  let fam := mkCIdentFrom (← getRef) ``TargetData
+  let idx := Name.quoteFrom id id.getId
+  `($[$doc?]? family_def $id : $fam $idx := $ty)
 
 /-- Macro for declaring new `CustomData`. -/
-scoped macro (name := customDataDecl) doc?:optional(Parser.Command.docComment)
-"custom_data " pkg:ident tgt:ident " : " ty:term : command => do
-  let dty := mkCIdentFrom (← getRef) ``CustomData
+scoped macro (name := customDataDecl)
+  doc?:optional(docComment) "custom_data " pkg:ident tgt:ident " : " ty:term
+: command => do
+  let fam := mkCIdentFrom (← getRef) ``CustomDataFam
   let id := mkIdentFrom tgt (pkg.getId ++ tgt.getId)
   let pkg := Name.quoteFrom pkg pkg.getId
   let tgt := Name.quoteFrom pkg tgt.getId
-  `($[$doc?]? family_def $id : $dty ($pkg, $tgt) := $ty)
+  `($[$doc?]? family_def $id : $fam ($pkg, $tgt) := $ty)
