src/lake/Lake/Config/FacetConfig.lean
@@ -11,25 +11,39 @@ namespace Lake
 open Lean (Name)
 
 /-- A facet's declarative configuration. -/
-structure FacetConfig (DataFam : Name → Type) (ι : Type) (name : Name) : Type where
+structure FacetConfig (kind name : Name) : Type where
   /-- The facet's fetch function. -/
-  fetchFn : ι → FetchM (Job (DataFam name))
+  fetchFn : TargetData kind → FetchM (Job (FacetData kind name))
   /-- Is this facet compatible with the `lake build` CLI? -/
   buildable : Bool := true
   /-- Format this facet's output (e.g., for `lake query`). -/
-  format : OutFormat → DataFam name → String
+  format : OutFormat → FacetData kind name → String
   deriving Inhabited
 
-protected abbrev FacetConfig.name (_ : FacetConfig DataFam ι name) := name
+protected abbrev FacetConfig.name (_ : FacetConfig kind name) := name
+
+/-- Run the facet configuration's fetch function. -/
+@[inline] def FacetConfig.run
+  [FamilyOut TargetData kind α]
+  [FamilyOut (FacetData kind) facet β]
+  (self : FacetConfig kind facet) (info : α)
+: FetchM (Job β) :=
+  cast (by simp) <| self.fetchFn <| toFamily info
 
 /-- A smart constructor for facet configurations that generate jobs for the CLI. -/
 @[inline] def mkFacetJobConfig
-  [FormatQuery α] [h : FamilyOut Fam facet α]
-  (build : ι → FetchM (Job α)) (buildable := true)
-: FacetConfig Fam ι facet where
+  [FormatQuery β]
+  [i : FamilyOut TargetData kind α]
+  [o : FamilyOut (FacetData kind) facet β]
+  (build : α → FetchM (Job β)) (buildable := true)
+: FacetConfig kind facet where
   buildable
-  fetchFn := h.family_key_eq_type ▸ build
-  format := h.family_key_eq_type ▸ formatQuery
+  fetchFn := i.fam_eq ▸ o.fam_eq ▸ build
+  format := o.fam_eq ▸ formatQuery
+
+/-- A two layer kind-name-configuration map of facets. -/
+abbrev FacetMap := DNameMap fun k => (DNameMap (FacetConfig k))
+@[inline] def FacetMap.empty : FacetMap := DNameMap.empty
 
 /-- A dependently typed configuration based on its registered name. -/
 structure NamedConfigDecl (β : Name → Type u) where
@@ -37,22 +51,31 @@ structure NamedConfigDecl (β : Name → Type u) where
   config : β name
 
 /-- A module facet's declarative configuration. -/
-abbrev ModuleFacetConfig := FacetConfig ModuleData Module
+abbrev ModuleFacetConfig := FacetConfig Module.facetKind
 
 /-- A module facet declaration from a configuration file. -/
 abbrev ModuleFacetDecl := NamedConfigDecl ModuleFacetConfig
 
 /-- A package facet's declarative configuration. -/
-abbrev PackageFacetConfig := FacetConfig PackageData Package
+abbrev PackageFacetConfig := FacetConfig Package.facetKind
 
 /-- A package facet declaration from a configuration file. -/
 abbrev PackageFacetDecl := NamedConfigDecl PackageFacetConfig
 
 /-- A library facet's declarative configuration. -/
-abbrev LibraryFacetConfig := FacetConfig LibraryData LeanLib
+abbrev LibraryFacetConfig := FacetConfig LeanLib.facetKind
 
 /-- A library facet declaration from a configuration file. -/
 abbrev LibraryFacetDecl := NamedConfigDecl LibraryFacetConfig
 
 deriving instance TypeName for
   ModuleFacetDecl, PackageFacetDecl, LibraryFacetDecl
+
+/-- A library facet's declarative configuration. -/
+abbrev LeanLibFacetConfig := LibraryFacetConfig
+
+/-- A Lean executable facet's declarative configuration. -/
+abbrev LeanExeFacetConfig := FacetConfig LeanExe.facetKind
+
+/-- An external library facet's declarative configuration. -/
+abbrev ExternLibFacetConfig := FacetConfig ExternLib.facetKind
