src/lake/Lake/Build/Target/Fetch.lean
@@ -9,29 +9,32 @@ import Lake.Config.Monad
 
 namespace Lake
 
-protected def BuildKey.fetch (self : BuildKey) [h : FamilyOut BuildData self α] : FetchM (Job α) := do
-  match self_eq:self with
-  | moduleFacet modName facetName =>
+private def BuildKey.fetchCore (self : BuildKey) : FetchM (Job (BuildData self)) := do
+  match self with
+  | module modName =>
     let some mod ← findModule? modName
       | error s!"invalid target '{self}': module '{modName}' not found in workspace"
-    have : FamilyOut BuildData (mod.facet facetName).key α :=
-      ⟨by simpa [self_eq] using h.family_key_eq_type⟩
-    fetch <| mod.facet facetName
-  | packageFacet pkgName facetName =>
+    return Job.pure <| toFamily mod
+  | package pkgName =>
     let some pkg ← findPackage? pkgName
       | error s!"invalid target '{self}': package '{pkgName}' not found in workspace"
-    have : FamilyOut BuildData (pkg.facet facetName).key α :=
-      ⟨by simpa [self_eq] using h.family_key_eq_type⟩
-    fetch <| pkg.facet facetName
-  | targetFacet pkgName targetName facetName =>
-    -- TODO: Support this
-    error s!"unsupported target {self}: fetching builtin targets by key is not currently supported"
-  | customTarget pkgName targetName =>
+    return Job.pure <| toFamily pkg.toPackage
+  | packageTarget pkgName target kind =>
     let some pkg ← findPackage? pkgName
       | error s!"invalid target '{self}': package '{pkgName}' not found in workspace"
-    have : FamilyOut BuildData (pkg.target targetName).key α :=
-      ⟨by simpa [self_eq] using h.family_key_eq_type⟩
-    fetch <| pkg.target targetName
+    fetch <| pkg.target target kind
+  | facet target facetName =>
+    if h : target.kind.isAnonymous then
+      error s!"invalid target '{self}': facet of opaque target kind '{target.kind}'"
+    else
+      let job ← target.fetchCore
+      let job : Job (TargetData target.kind) :=
+        cast (by rw [target.data_eq_of_kind h]) job
+      job.bindM fun data => fetch (.facet target data facetName)
+
+@[inline] protected def BuildKey.fetch
+  (self : BuildKey) [FamilyOut BuildData self α] : FetchM (Job α)
+:= cast (by simp) self.fetchCore
 
 @[inline] protected def Target.fetch (self : Target α) : FetchM (Job α) := do
  have := self.data_def; self.key.fetch
